Fix a big issue with readDirents
We no longer read the entire directory and then close it; we instead
need to leave it open for future directory operations, and close it only
after reading or writing to it.

One unfortunate side effect of this requirement is that we cannot have a
directory and file open at the same time; most of the time this is fine,
but it must be managed correctly by every operation.

src/Dafny/examples/fs/mem_dirent.dfy
@@ -266,6 +266,35 @@ module MemDirEntries
       file.fs.has_jrnl(txn)
     }
 
+    predicate inode_unchanged()
+      reads file.fs.fs.fs.fs, file.i.Repr
+      requires file.i.Valid()
+    {
+      file.fs.inode_unchanged(file.ino, file.i.val())
+    }
+
+    method finishReadonly()
+      modifies file.fs.fs.fs.fs
+      requires Valid()
+      requires (reveal file.ValidFs(); inode_unchanged())
+      ensures file.fs.Valid()
+    {
+      reveal file.ValidFs();
+      file.fs.finishInodeReadonly(file.ino, file.i);
+    }
+
+    method finish(txn: Txn)
+      modifies file.ReprFs
+      requires has_jrnl(txn)
+      requires Valid()
+      ensures file.fs.Valid()
+      ensures file.fs.types_unchanged()
+      ensures file.fs.data == old(file.fs.data)
+    {
+      reveal file.ValidFs();
+      file.fs.finishInode(txn, file.ino, file.i);
+    }
+
     method loadDirOff(txn: Txn, k: uint64)
       modifies file
       requires Valid() ensures Valid()
